checkpoint updated manual wp_Encode wp_Decode

testdata/out/coq/completeslice_proof.v
@@ -27,24 +27,10 @@ Definition has_encoding (encoded:list u8) (args:C) : Prop :=
               (u64_le $ length $ args.(strg2)) ++ args.(strg2) ++
               (u64_le $ length $ args.(bytes)) ++ args.(bytes).
 
-Definition own_byte (v: val) (b: u8) (dq: dfrac) : iProp Σ :=
-  ⌜v = to_val b⌝.
-
 Definition own (args__v: val) (args__c: C) (dq: dfrac) : iProp Σ :=
   ∃(bytes_sl : Slice.t), 
   "%Hown_struct" ∷ ⌜ args__v = (#(str args__c.(strg)), (#(str args__c.(strg2)), (slice_val bytes_sl, #())))%V ⌝ ∗
-  "Hown_bytes" ∷ is_pred_slice own_byte bytes_sl byteT dq args__c.(bytes).
-
-Instance val_IntoVal : IntoVal val.
-Proof.
-  refine {|
-      to_val := λ v, v;
-      from_val := λ v, Some v;
-      IntoVal_def := #();
-    |}.
-  intros v; auto.
-Defined.
-
+  "Hown_bytes" ∷ is_pred_slice own_val bytes_sl byteT dq args__c.(bytes).
 
 Lemma wp_Encode (args__v : val) (args__c : C) (pre_sl : Slice.t) (prefix : list u8) (dq : dfrac):
   {{{
@@ -64,7 +50,9 @@ Proof.
   wp_rec. wp_pures.
   iUnfold own in "Hown". iNamed "Hown". rewrite Hown_struct.
   iUnfold is_pred_slice in "Hown_bytes".
-  iDestruct "Hown_bytes" as "[%vs [Hown_bytes HΨ_bytes]]".
+  iDestruct "Hown_bytes" as "[%vs [Hown_bytes #HΨ_bytes]]".
+  iDestruct (big_sepL2_length with "HΨ_bytes") as "%HΨ_bytes_len".
+  iDestruct (big_sepL2_own_val with "HΨ_bytes") as "%HΨ_bytes_rel".
   wp_apply (wp_ref_to); first by val_ty.
   iIntros (?) "Hptr". wp_pures.
 
@@ -84,28 +72,31 @@ Proof.
   wp_load. wp_apply (wp_WriteBytes with "[$Hsl $Hargs_strg2_enc]").
   iIntros (?) "[Hsl _]". wp_store.
 
-  iDestruct (slice.own_slice_small_sz with "Hown_bytes") as "%Hargs_bytes_sz".
+  iDestruct (own_slice_small_sz with "Hown_bytes") as "%Hargs_bytes_sz".
   wp_pures. wp_apply (wp_slice_len). wp_load.
   wp_apply (wp_WriteInt with "[$Hsl]"). iIntros (?) "Hsl". wp_store.
   wp_pures. wp_load.
   wp_apply (wp_WriteBytes with "[$Hsl Hown_bytes]").
-  { iUnfold own_slice_small.  }
-  iIntros (?) "[Hsl Hargs_bytes_sl]". wp_store.
+  { rewrite -> HΨ_bytes_rel.
+    unfold own_slice_small.
+    rewrite untype_val_list.
+    iFrame. }
+  iIntros (?) "[Hsl Hargs_bytes_sl]". wp_store. 
 
 
   wp_load. iApply "HΦ". iModIntro. rewrite -?app_assoc.
-  iFrame. iPureIntro.
-
-  unfold has_encoding. split.
-  {
-  
-  rewrite ?string_bytes_length.
-  rewrite Hargs_strg_sz.
-  rewrite Hargs_strg2_sz.
-  rewrite Hargs_bytes_sz.
-  rewrite ?w64_to_nat_id. exact.
-
-  } done.
+  iFrame. iSplitR.
+  + iPureIntro.
+    unfold has_encoding.
+    rewrite ?string_bytes_length.
+    rewrite Hargs_strg_sz.
+    rewrite Hargs_strg2_sz.
+    rewrite <- HΨ_bytes_len.
+    rewrite Hargs_bytes_sz.
+    rewrite ?w64_to_nat_id. exact.
+  + iExists bytes_sl. iSplitR; first done.
+    iUnfold is_pred_slice. unfold own_slice_small. iExists (list.untype args__c.(bytes)).
+    rewrite untype_val_list. iFrame. rewrite HΨ_bytes_rel. done.
 Qed.
 
 Lemma wp_Decode (enc : list u8) (enc_sl : Slice.t) (args__c : C) (suffix : list u8) (dq : dfrac):
@@ -182,7 +173,12 @@ Proof.
 
   wp_load. wp_load. wp_load. wp_load.
   wp_pures. iApply "HΦ". iModIntro. rewrite ?string_to_bytes_to_string. iFrame.
-  iPureIntro. reflexivity.
+  iUnfold own. iExists b1. iSplitR; first done. iUnfold is_pred_slice.
+  iExists (list.untype args__c.(bytes)). iSplitR "Hbytes".
+  + unfold own_slice_small. rewrite untype_val_list. iFrame.
+  + unfold list.untype, own_val.
+    rewrite big_sepL2_fmap_l.
+    rewrite <- big_sepL_sepL2_diag. done.
 Qed.
 
 End completeSlice.
